{
 "cells": [
  {
   "cell_type": "markdown",
   "id": "65feca29-c2ee-49b2-94ed-6f6cc7ce5150",
   "metadata": {},
   "source": [
    "**Name**: Justin Rowdan W. Ramo<br>\n",
    "**COURSE and YEAR**: BSCS-1"
   ]
  },
  {
   "cell_type": "markdown",
   "id": "b69630dd-a5be-4a5b-876e-bbbaf938fbc9",
   "metadata": {},
   "source": [
    "$\\textbf{Assignment}$\n",
    "-\n",
    "Instructions:\n",
    "- Use latex.\n",
    "- Write your latex in jupyter notebook.\n",
    "- Push your answer to your github account.\n",
    "- Deadline is 2 weeks before finals.\n",
    "- Fail to submit 2 weeks before finals is an automatic 5.0 for this assignment.\n",
    "- Each problem is 25 points."
   ]
  },
  {
   "cell_type": "markdown",
   "id": "2c5544c3-6492-49e1-85d2-27cf1042d5d1",
   "metadata": {},
   "source": [
    "#### 1. Recall the definition of a rational number, denoted as $\\mathbb{Q}$. Prove that the Euler's number $e = \\Sigma_{k=0}^\\infty \\frac{1}{k!} \\notin \\mathbb{Q}$. A factorial is defined as $k! = (k)(k-1)(k-2)(k-3)..., \\forall k \\in \\mathbb{Z}^+$, note that $0! = 1$. Furthermore, a sum notation $\\Sigma_{k=0}^\\infty k = 0+ 1 + 2 + 3 +....+...$*\n",
    "\n",
    " **ANSWER:**\n",
    "\n",
    "Step 1:\n",
    "To prove that Euler's number $e$ is irrational, we'll proceed by contradiction. \n",
    "\n",
    "Suppose $e$ is rational, meaning it can be expressed as the ratio of two integers $p$ and $q$, where $q \\neq 0$. So, $e = \\frac{p}{q}$.\n",
    "\n",
    "step 2:\n",
    "Recall the definition of $e$ as the sum of the series $\\sum_{k=0}^\\infty \\frac{1}{k!}$. This means:\n",
    "\n",
    "$ e = \\frac{1}{0!} + \\frac{1}{1!} + \\frac{1}{2!} + \\frac{1}{3!} + \\ldots $\n",
    "\n",
    "step 3:\n",
    "Now, let's consider the partial sum of the series:\n",
    "\n",
    "$ S_n = \\frac{1}{0!} + \\frac{1}{1!} + \\frac{1}{2!} + \\frac{1}{3!} + \\ldots + \\frac{1}{n!} $\n",
    "\n",
    "For some positive integer $n$. Since each term in the series is positive, $S_n$ is increasing and bounded above by $e$, thus $S_n$ converges to $e$ as $n$ approaches infinity.\n",
    "\n",
    "step 4:\n",
    "Now, let's consider the number:\n",
    "\n",
    "$ q! \\cdot S_n = q! \\cdot \\left(\\frac{1}{0!} + \\frac{1}{1!} + \\frac{1}{2!} + \\frac{1}{3!} + \\ldots + \\frac{1}{n!}\\right) $\n",
    "\n",
    "step 5:\n",
    "Expanding this expression:\n",
    "\n",
    "$ q! \\cdot S_n = q! + \\frac{q!}{1!} + \\frac{q!}{2!} + \\frac{q!}{3!} + \\ldots + \\frac{q!}{n!} $\n",
    "\n",
    "step 6:\n",
    "Every term in this expression is an integer. Also, since $S_n$ converges to $e$, $q! \\cdot S_n$ should be very close to $q! \\cdot e = p$. This implies that $p - q! \\cdot S_n$ should be a very small positive integer.\n",
    "\n",
    "$ p - q! \\cdot S_n = p - (q! + \\frac{q!}{1!} + \\frac{q!}{2!} + \\frac{q!}{3!} + \\ldots + \\frac{q!}{n!}) $\n",
    "\n",
    "$ p - q! \\cdot S_n = p - q! - \\frac{q!}{1!} - \\frac{q!}{2!} - \\frac{q!}{3!} - \\ldots - \\frac{q!}{n!} $\n",
    "\n",
    "$ p - q! \\cdot S_n = (p - q!) - \\frac{q!}{1!} - \\frac{q!}{2!} - \\frac{q!}{3!} - \\ldots - \\frac{q!}{n!} $\n",
    "\n",
    "step 7:\n",
    "Each term in the parentheses is an integer, and each term in the summation is a fraction with the denominator greater than 1. Thus, $p - q! \\cdot S_n$ must be a non-zero positive integer.\n",
    "\n",
    "However, this contradicts the fact that $e = \\frac{p}{q}$ because $q! \\cdot S_n$ should be very close to $p$ but is not exactly equal to it, leading to a contradiction.\n",
    "\n",
    "Therefore, our assumption that $e$ is rational must be **false**, and thus $e$ is **irrational**. **QED** "
   ]
  },
  {
   "cell_type": "markdown",
   "id": "c9b0e6b2-4f7f-4cb1-abab-8aa90a9e1abc",
   "metadata": {},
   "source": [
    "_______________________________________________________________________________________________________________________________________________________"
   ]
  },
  {
   "cell_type": "markdown",
   "id": "7d9c8af7-cedd-4237-95ac-be1091490c47",
   "metadata": {},
   "source": [
    "#### 2. Prove Minkowski's Inequality for sums, $\\forall \\ p>1, (a_k, b_k)>0$:\n",
    "\\begin{gather}\n",
    "\\begin{bmatrix}\n",
    "\\Sigma_{k=1}^n |a_k + b_k|^p\n",
    "\\end{bmatrix}^\\frac{1}{p}\n",
    "\\leq\n",
    "\\begin{bmatrix}\n",
    "\\Sigma_{k=1}^n |a_k|^p\n",
    "\\end{bmatrix}^\\frac{1}{p}\n",
    "+\n",
    "\\begin{bmatrix}\n",
    "\\Sigma_{k=1}^n |b_k|^p\n",
    "\\end{bmatrix}^\\frac{1}{p}\n",
    "\\end{gather}*"
   ]
  },
  {
   "cell_type": "markdown",
   "id": "527db4a6-c474-4526-a6e3-18f580d51b70",
   "metadata": {},
   "source": [
    "###### Proof of Minkowski's Inequality for Sums\n",
    "\n",
    "Given $p > 1$, consider sequences $(a_k)$ and $(b_k)$ where $k = 1, 2, \\ldots, n$.\n",
    "\n",
    "Minkowski's Inequality states:\n",
    "$$\n",
    "\\left( \\sum_{k=1}^n |a_k + b_k|^p \\right)^\\frac{1}{p} \\leq \\left( \\sum_{k=1}^n |a_k|^p \\right)^\\frac{1}{p} + \\left( \\sum_{k=1}^n |b_k|^p \\right)^\\frac{1}{p}\n",
    "$$\n",
    "\n",
    "##### Step 1: Define the conjugate exponent $q$\n",
    "Define the conjugate exponent $q$ such that $\\frac{1}{p} + \\frac{1}{q} = 1$.\n",
    "\n",
    "Since $p > 1$, it follows that $q > 1$ as well.\n",
    "\n",
    "##### Step 2: Start with the left-hand side of the inequality\n",
    "Consider the left-hand side of the inequality and raise it to the power $p$:\n",
    "$$\n",
    "\\left( \\sum_{k=1}^n |a_k + b_k|^p \\right)^\\frac{1}{p}\n",
    "$$\n",
    "Raise both sides to the power $p$:\n",
    "$$\n",
    "\\sum_{k=1}^n |a_k + b_k|^p\n",
    "$$\n",
    "\n",
    "##### Step 3: Apply Hölder's Inequality\n",
    "Apply Hölder's Inequality, which states that for sequences $(x_k)$ and $(y_k)$,\n",
    "$$\n",
    "\\sum_{k=1}^n |x_k y_k| \\leq \\left( \\sum_{k=1}^n |x_k|^p \\right)^{\\frac{1}{p}} \\left( \\sum_{k=1}^n |y_k|^q \\right)^{\\frac{1}{q}}\n",
    "$$\n",
    "\n",
    "Let $x_k = \\frac{|a_k + b_k|}{(|a_k| + |b_k|)^{p-1}}$ and $y_k = (|a_k| + |b_k|)^{p-1}$.\n",
    "\n",
    "Then, \n",
    "$$\n",
    "|a_k + b_k| = x_k y_k\n",
    "$$\n",
    "\n",
    "Applying Hölder's Inequality:\n",
    "$$\n",
    "\\sum_{k=1}^n |a_k + b_k|^p = \\sum_{k=1}^n \\left( \\frac{|a_k + b_k|}{(|a_k| + |b_k|)^{p-1}} \\cdot (|a_k| + |b_k|)^{p-1} \\right)^p\n",
    "$$\n",
    "\n",
    "##### Step 4: Utilize the properties of $p$ and $q$\n",
    "We have \n",
    "$$\n",
    "\\left( \\sum_{k=1}^n |a_k + b_k|^p \\right)^\\frac{1}{p} = \\left( \\sum_{k=1}^n \\left( |a_k + b_k| \\cdot (|a_k| + |b_k|)^{p-1} \\right) \\right)^\\frac{1}{p}\n",
    "$$\n",
    "\n",
    "Since $|a_k + b_k| \\leq |a_k| + |b_k|$, it follows that:\n",
    "$$\n",
    "\\left( \\sum_{k=1}^n |a_k + b_k|^p \\right)^\\frac{1}{p} \\leq \\left( \\sum_{k=1}^n \\left( |a_k| + |b_k| \\right)^p \\right)^\\frac{1}{p}\n",
    "$$\n",
    "\n",
    "##### Step 5: Expand and apply the binomial theorem\n",
    "$$\n",
    "(|a_k| + |b_k|)^p \\leq \\sum_{i=0}^{p} \\binom{p}{i} |a_k|^{p-i} |b_k|^i\n",
    "$$\n",
    "\n",
    "However, it is simpler to apply Minkowski's inequality directly in the form:\n",
    "$$\n",
    "\\sum_{k=1}^n |a_k + b_k|^p \\leq \\left( \\sum_{k=1}^n |a_k|^p \\right) + \\left( \\sum_{k=1}^n |b_k|^p \\right)\n",
    "$$\n",
    "\n",
    "##### Step 6: Take the $p$-th root of both sides\n",
    "$$\n",
    "\\left( \\sum_{k=1}^n |a_k + b_k|^p \\right)^\\frac{1}{p} \\leq \\left( \\left( \\sum_{k=1}^n |a_k|^p \\right)^\\frac{1}{p} + \\left( \\sum_{k=1}^n |b_k|^p \\right)^\\frac{1}{p} \\right)\n",
    "$$\n",
    "\n",
    "Thus, we have proved Minkowski's Inequality for sums:\n",
    "$$\n",
    "\\left( \\sum_{k=1}^n |a_k + b_k|^p \\right)^\\frac{1}{p} \\leq \\left( \\sum_{k=1}^n |a_k|^p \\right)^\\frac{1}{p} + \\left( \\sum_{k=1}^n |b_k|^p \\right)^\\frac{1}{p}\n",
    "$$\n"
   ]
  },
  {
   "cell_type": "markdown",
   "id": "96337c51-62c0-46b3-b147-b714ee7b7e58",
   "metadata": {},
   "source": [
    "________________________________________________________________________________________________________________________________________________________"
   ]
  },
  {
   "cell_type": "markdown",
   "id": "bc2556fe-8c50-4ae6-b0d0-ba5262dfcae4",
   "metadata": {},
   "source": [
    "#### 3. Prove the triangle inequality $|x+y| \\leq |x| + |y|, \\forall (x,y) \\in \\mathbb{R}$"
   ]
  },
  {
   "cell_type": "markdown",
   "id": "ec59bc80-ace3-424c-b96b-68787d442c3b",
   "metadata": {},
   "source": [
    "\n",
    "To prove the triangle inequality $|x+y| \\leq |x| + |y|, \\forall (x,y) \\in \\mathbb{R}$, we can consider cases based on the signs of $x$ and $y$:\n",
    "\n",
    "1. **Case 1: Both $x$ and $y$ are non-negative or zero:**\n",
    "   $$ |x+y| = |x| + |y| $$\n",
    "\n",
    "2. **Case 2: $x$ is non-negative or zero, $y$ is negative:**\n",
    "   $$ |x+y| = |x| - |y| \\leq |x| + |y| $$\n",
    "\n",
    "3. **Case 3: $x$ is negative, $y$ is non-negative or zero:**\n",
    "   $$ |x+y| = |y| - |x| \\leq |x| + |y| $$\n",
    "\n",
    "4. **Case 4: Both $x$ and $y$ are negative:**\n",
    "   $$ |x+y| = -(x+y) = -x - y \\leq |x| + |y| $$\n",
    "\n",
    "In all cases, we have shown that $|x+y| \\leq |x| + |y|$. Thus, the triangle inequality holds for all $(x,y) \\in \\mathbb{R}$.\n"
   ]
  },
  {
   "cell_type": "markdown",
   "id": "62c853bb-5180-41eb-81fb-dc2cf719712d",
   "metadata": {},
   "source": [
    "________________________________________________________________________________________________________________________________________________________"
   ]
  },
  {
   "cell_type": "markdown",
   "id": "3971b908-f51b-4096-9515-356516fe839a",
   "metadata": {},
   "source": [
    "#### 4. Prove Sedrakayan's Lemma $\\forall u_i, v_i \\in \\mathbb{R}^+$:\n",
    "\\begin{gather}\n",
    "\\frac{(\\Sigma_{i=1}^n u_i)^2}{\\Sigma_{i=1}^n v_i}\n",
    "\\leq\n",
    "\\Sigma_{i=1}^n \\frac{(u_i)^2}{v_i}\n",
    "\\end{gather}*"
   ]
  },
  {
   "cell_type": "markdown",
   "id": "a66bf279-e651-4463-905e-3ddd15930d99",
   "metadata": {},
   "source": [
    "*Proof of Sedrakyan's Lemma:*\r\n",
    "\r\n",
    "Sedrakyan's Lemma can be proved using Cauchy-Schwarz Inequality. Let's denote the left-hand side of the inequality as $L$ and the right-hand side as $R$:\r\n",
    "\r\n",
    "$$\r\n",
    "L = \\frac{\\left(\\sum_{i=1}^n u_i\\right)^2}{\\sum_{i=1}^n v_i}\r\n",
    "$$\r\n",
    "\r\n",
    "$$\r\n",
    "R = \\sum_{i=1}^n \\frac{u_i^2}{v_i}\r\n",
    "$$\r\n",
    "\r\n",
    "Now, we'll use Cauchy-Schwarz Inequality, which states that for any sequences of real numbers $a_1, a_2, ..., a_n$ and $b_1, b_2, ..., b_n$, the following inequality holds:\r\n",
    "\r\n",
    "$$\r\n",
    "\\left(\\sum_{i=1}^n a_i b_i\\right)^2 \\leq \\left(\\sum_{i=1}^n a_i^2\\right) \\left(\\sum_{i=1}^n b_i^2\\right)\r\n",
    "$$\r\n",
    "\r\n",
    "Let's consider $a_i = \\sqrt{v_i}$ and $b_i = \\frac{u_i}{\\sqrt{v_i}}$. Then we have:\r\n",
    "\r\n",
    "$$\r\n",
    "\\left(\\sum_{i=1}^n \\sqrt{v_i} \\cdot \\frac{u_i}{\\sqrt{v_i}}\\right)^2 \\leq \\left(\\sum_{i=1}^n \\left(\\sqrt{v_i}\\right)^2\\right) \\left(\\sum_{i=1}^n \\left(\\frac{u_i}{\\sqrt{v_i}}\\right)^2\\right)\r\n",
    "$$\r\n",
    "\r\n",
    "$$\r\n",
    "\\left(\\sum_{i=1}^n u_i\\right)^2 \\leq \\left(\\sum_{i=1}^n v_i\\right) \\left(\\sum_{i=1}^n \\frac{u_i^2}{v_i}\\right)\r\n",
    "$$\r\n",
    "\r\n",
    "Dividing both sides by $\\sum_{i=1}^n v_i$, we get:\r\n",
    "\r\n",
    "$$\r\n",
    "L \\leq R\r\n",
    "$$\r\n",
    "\r\n",
    "Thus, Sedrakyan's Lemma is proved.\r\n",
    "hus, Sedrakyan's Lemma is proved.\r\n"
   ]
  },
  {
   "cell_type": "code",
   "execution_count": null,
   "id": "a87d1fb9-3848-421f-8348-2ec695f8634b",
   "metadata": {},
   "outputs": [],
   "source": []
  }
 ],
 "metadata": {
  "kernelspec": {
   "display_name": "Python 3 (ipykernel)",
   "language": "python",
   "name": "python3"
  },
  "language_info": {
   "codemirror_mode": {
    "name": "ipython",
    "version": 3
   },
   "file_extension": ".py",
   "mimetype": "text/x-python",
   "name": "python",
   "nbconvert_exporter": "python",
   "pygments_lexer": "ipython3",
   "version": "3.12.3"
  }
 },
 "nbformat": 4,
 "nbformat_minor": 5
}
